HOL/DataStrs/BST.thy
@@ -17,27 +17,27 @@ subsection \<open>Definition and setup for trees\<close>
 datatype ('a, 'b) tree =
     Tip | Node (lsub: "('a, 'b) tree") (key: 'a) (nval: 'b) (rsub: "('a, 'b) tree")
 
-setup {* add_resolve_prfstep @{thm tree.distinct(1)} *}
-setup {* fold add_rewrite_rule @{thms tree.sel} *}
-setup {* add_forward_prfstep @{thm tree.collapse} *}
-setup {* add_var_induct_rule @{thm tree.induct} *}
+setup \<open>add_resolve_prfstep @{thm tree.distinct(1)}\<close>
+setup \<open>fold add_rewrite_rule @{thms tree.sel}\<close>
+setup \<open>add_forward_prfstep @{thm tree.collapse}\<close>
+setup \<open>add_var_induct_rule @{thm tree.induct}\<close>
 
 subsection \<open>Inorder traversal, and set of elements of a tree\<close>
 
 fun in_traverse :: "('a, 'b) tree \<Rightarrow> 'a list" where
   "in_traverse Tip = []"
 | "in_traverse (Node l k v r) = in_traverse l @ k # in_traverse r"
-setup {* fold add_rewrite_rule @{thms in_traverse.simps} *}
+setup \<open>fold add_rewrite_rule @{thms in_traverse.simps}\<close>
 
 fun tree_set :: "('a, 'b) tree \<Rightarrow> 'a set" where
   "tree_set Tip = {}"
 | "tree_set (Node l k v r) = {k} \<union> tree_set l \<union> tree_set r"
-setup {* fold add_rewrite_rule @{thms tree_set.simps} *}
+setup \<open>fold add_rewrite_rule @{thms tree_set.simps}\<close>
 
 fun in_traverse_pairs :: "('a, 'b) tree \<Rightarrow> ('a \<times> 'b) list" where
   "in_traverse_pairs Tip = []"
 | "in_traverse_pairs (Node l k v r) = in_traverse_pairs l @ (k, v) # in_traverse_pairs r"
-setup {* fold add_rewrite_rule @{thms in_traverse_pairs.simps} *}
+setup \<open>fold add_rewrite_rule @{thms in_traverse_pairs.simps}\<close>
 
 lemma in_traverse_fst [rewrite]:
   "map fst (in_traverse_pairs t) = in_traverse t"
@@ -45,7 +45,7 @@ lemma in_traverse_fst [rewrite]:
 
 definition tree_map :: "('a, 'b) tree \<Rightarrow> ('a, 'b) map" where
   "tree_map t = map_of_alist (in_traverse_pairs t)"
-setup {* add_rewrite_rule @{thm tree_map_def} *}
+setup \<open>add_rewrite_rule @{thm tree_map_def}\<close>
 
 subsection \<open>Sortedness on trees\<close>
 
@@ -53,7 +53,7 @@ fun tree_sorted :: "('a::linorder, 'b) tree \<Rightarrow> bool" where
   "tree_sorted Tip = True"
 | "tree_sorted (Node l k v r) = ((\<forall>x\<in>tree_set l. x < k) \<and> (\<forall>x\<in>tree_set r. k < x)
                               \<and> tree_sorted l \<and> tree_sorted r)"
-setup {* fold add_rewrite_rule @{thms tree_sorted.simps} *}
+setup \<open>fold add_rewrite_rule @{thms tree_sorted.simps}\<close>
 
 lemma tree_sorted_lr [forward]:
   "tree_sorted (Node l k v r) \<Longrightarrow> tree_sorted l \<and> tree_sorted r" by auto2
@@ -67,7 +67,7 @@ lemma inorder_pairs_sorted [rewrite]:
 @proof @induct t @qed
 
 (* Use definition in terms of in_traverse from now on. *)
-setup {* fold del_prfstep_thm (@{thms tree_set.simps} @ @{thms tree_sorted.simps}) *}
+setup \<open>fold del_prfstep_thm (@{thms tree_set.simps} @ @{thms tree_sorted.simps})\<close>
 
 subsection \<open>Rotation on trees\<close>
 
@@ -95,7 +95,7 @@ fun tree_insert :: "'a::ord \<Rightarrow> 'b \<Rightarrow> ('a, 'b) tree \<Right
     (if x = y then Node l x v r
      else if x < y then Node (tree_insert x v l) y w r
      else Node l y w (tree_insert x v r))"
-setup {* fold add_rewrite_rule @{thms tree_insert.simps} *}
+setup \<open>fold add_rewrite_rule @{thms tree_insert.simps}\<close>
  
 lemma insert_in_traverse_pairs [rewrite]:
   "tree_sorted t \<Longrightarrow> in_traverse_pairs (tree_insert x v t) = ordered_insert_pairs x v (in_traverse_pairs t)"
@@ -114,7 +114,7 @@ fun del_min :: "('a, 'b) tree \<Rightarrow> ('a \<times> 'b) \<times> ('a, 'b) t
 | "del_min (Node lt x v rt) =
    (if lt = Tip then ((x, v), rt) else
     (fst (del_min lt), Node (snd (del_min lt)) x v rt))"
-setup {* add_rewrite_rule @{thm del_min.simps(2)} *}
+setup \<open>add_rewrite_rule @{thm del_min.simps(2)}\<close>
 
 lemma delete_min_del_hd_pairs [rewrite]:
   "t \<noteq> Tip \<Longrightarrow> fst (del_min t) # in_traverse_pairs (snd (del_min t)) = in_traverse_pairs t"
@@ -125,7 +125,7 @@ fun delete_elt_tree :: "('a, 'b) tree \<Rightarrow> ('a, 'b) tree" where
 | "delete_elt_tree (Node lt x v rt) =
     (if lt = Tip then rt else if rt = Tip then lt else
      Node lt (fst (fst (del_min rt))) (snd (fst (del_min rt))) (snd (del_min rt)))"
-setup {* add_rewrite_rule @{thm delete_elt_tree.simps(2)} *}
+setup \<open>add_rewrite_rule @{thm delete_elt_tree.simps(2)}\<close>
 
 lemma delete_elt_in_traverse_pairs [rewrite]:
   "in_traverse_pairs (delete_elt_tree (Node lt x v rt)) = in_traverse_pairs lt @ in_traverse_pairs rt" by auto2
@@ -136,7 +136,7 @@ fun tree_delete :: "'a::ord \<Rightarrow> ('a, 'b) tree \<Rightarrow> ('a, 'b) t
     (if x = y then delete_elt_tree (Node l y w r)
      else if x < y then Node (tree_delete x l) y w r
      else Node l y w (tree_delete x r))"
-setup {* fold add_rewrite_rule @{thms tree_delete.simps} *}
+setup \<open>fold add_rewrite_rule @{thms tree_delete.simps}\<close>
 
 lemma tree_delete_in_traverse_pairs [rewrite]:
   "tree_sorted t \<Longrightarrow> in_traverse_pairs (tree_delete x t) = remove_elt_pairs x (in_traverse_pairs t)"
@@ -156,7 +156,7 @@ fun tree_search :: "('a::ord, 'b) tree \<Rightarrow> 'a \<Rightarrow> 'b option"
   (if x = k then Some v
    else if x < k then tree_search l x
    else tree_search r x)"
-setup {* fold add_rewrite_rule @{thms tree_search.simps} *}
+setup \<open>fold add_rewrite_rule @{thms tree_search.simps}\<close>
 
 theorem tree_search_correct [rewrite]:
   "tree_sorted t \<Longrightarrow> tree_search t x = (tree_map t)\<langle>x\<rangle>"
