HOL/DataStrs/Interval_Tree.thy
@@ -22,28 +22,28 @@ datatype interval_tree =
 where
   "tmax Tip = 0"
 
-setup {* add_resolve_prfstep @{thm interval_tree.distinct(1)} *}
-setup {* fold add_rewrite_rule @{thms interval_tree.sel} *}
-setup {* add_forward_prfstep @{thm interval_tree.collapse} *}
-setup {* add_var_induct_rule @{thm interval_tree.induct} *}
+setup \<open>add_resolve_prfstep @{thm interval_tree.distinct(1)}\<close>
+setup \<open>fold add_rewrite_rule @{thms interval_tree.sel}\<close>
+setup \<open>add_forward_prfstep @{thm interval_tree.collapse}\<close>
+setup \<open>add_var_induct_rule @{thm interval_tree.induct}\<close>
 
 subsection \<open>Inorder traversal, and set of elements of a tree\<close>
 
 fun in_traverse :: "interval_tree \<Rightarrow> nat idx_interval list" where
   "in_traverse Tip = []"
 | "in_traverse (Node l it m r) = in_traverse l @ it # in_traverse r"
-setup {* fold add_rewrite_rule @{thms in_traverse.simps} *}
+setup \<open>fold add_rewrite_rule @{thms in_traverse.simps}\<close>
 
 fun tree_set :: "interval_tree \<Rightarrow> nat idx_interval set" where
   "tree_set Tip = {}"
 | "tree_set (Node l it m r) = {it} \<union> tree_set l \<union> tree_set r"
-setup {* fold add_rewrite_rule @{thms tree_set.simps} *}
+setup \<open>fold add_rewrite_rule @{thms tree_set.simps}\<close>
 
 fun tree_sorted :: "interval_tree \<Rightarrow> bool" where
   "tree_sorted Tip = True"
 | "tree_sorted (Node l it m r) = ((\<forall>x\<in>tree_set l. x < it) \<and> (\<forall>x\<in>tree_set r. it < x)
                                    \<and> tree_sorted l \<and> tree_sorted r)"
-setup {* fold add_rewrite_rule @{thms tree_sorted.simps} *}
+setup \<open>fold add_rewrite_rule @{thms tree_sorted.simps}\<close>
 
 lemma tree_sorted_lr [forward]:
   "tree_sorted (Node l it m r) \<Longrightarrow> tree_sorted l \<and> tree_sorted r" by auto2
@@ -63,7 +63,7 @@ lemma inorder_sorted [rewrite]:
 @proof @induct t @qed
 
 (* Use definition in terms of in_traverse from now on. *)
-setup {* fold del_prfstep_thm (@{thms tree_set.simps} @ @{thms tree_sorted.simps}) *}
+setup \<open>fold del_prfstep_thm (@{thms tree_set.simps} @ @{thms tree_sorted.simps})\<close>
 
 subsection \<open>Invariant on the maximum\<close>
 
@@ -73,7 +73,7 @@ definition max3 :: "nat idx_interval \<Rightarrow> nat \<Rightarrow> nat \<Right
 fun tree_max_inv :: "interval_tree \<Rightarrow> bool" where
   "tree_max_inv Tip = True"
 | "tree_max_inv (Node l it m r) \<longleftrightarrow> (tree_max_inv l \<and> tree_max_inv r \<and> m = max3 it (tmax l) (tmax r))"
-setup {* fold add_rewrite_rule @{thms tree_max_inv.simps} *}
+setup \<open>fold add_rewrite_rule @{thms tree_max_inv.simps}\<close>
 
 lemma tree_max_is_max [resolve]:
   "tree_max_inv t \<Longrightarrow> it \<in> tree_set t \<Longrightarrow> high (int it) \<le> tmax t"
@@ -91,7 +91,7 @@ lemma tmax_exists [backward]:
 (* For insertion *)
 lemma max3_insert [rewrite]: "max3 it 0 0 = high (int it)" by auto2
 
-setup {* del_prfstep_thm @{thm max3_def} *}
+setup \<open>del_prfstep_thm @{thm max3_def}\<close>
 
 subsection \<open>Condition on the values\<close>
 
@@ -116,7 +116,7 @@ fun insert :: "nat idx_interval \<Rightarrow> interval_tree \<Rightarrow> interv
      else
        let r' = insert x r in
            Node l y (max3 y (tmax l) (tmax r')) r')"
-setup {* fold add_rewrite_rule @{thms insert.simps} *}
+setup \<open>fold add_rewrite_rule @{thms insert.simps}\<close>
 
 lemma tree_insert_in_traverse [rewrite]:
   "tree_sorted t \<Longrightarrow> in_traverse (insert x t) = ordered_insert x (in_traverse t)"
@@ -140,13 +140,13 @@ fun del_min :: "interval_tree \<Rightarrow> nat idx_interval \<times> interval_t
    (if lt = Tip then (v, rt) else
     let lt' = snd (del_min lt) in
     (fst (del_min lt), Node lt' v (max3 v (tmax lt') (tmax rt)) rt))"
-setup {* add_rewrite_rule @{thm del_min.simps(2)} *}
-setup {* register_wellform_data ("del_min t", ["t \<noteq> Tip"]) *}
+setup \<open>add_rewrite_rule @{thm del_min.simps(2)}\<close>
+setup \<open>register_wellform_data ("del_min t", ["t \<noteq> Tip"])\<close>
 
 lemma delete_min_del_hd:
   "t \<noteq> Tip \<Longrightarrow> fst (del_min t) # in_traverse (snd (del_min t)) = in_traverse t"
 @proof @induct t @qed
-setup {* add_forward_prfstep_cond @{thm delete_min_del_hd} [with_term "in_traverse (snd (del_min ?t))"] *}
+setup \<open>add_forward_prfstep_cond @{thm delete_min_del_hd} [with_term "in_traverse (snd (del_min ?t))"]\<close>
 
 lemma delete_min_max_inv [forward_arg]:
   "tree_max_inv t \<Longrightarrow> t \<noteq> Tip \<Longrightarrow> tree_max_inv (snd (del_min t))"
@@ -154,7 +154,7 @@ lemma delete_min_max_inv [forward_arg]:
 
 lemma delete_min_on_set:
   "t \<noteq> Tip \<Longrightarrow> {fst (del_min t)} \<union> tree_set (snd (del_min t)) = tree_set t" by auto2
-setup {* add_forward_prfstep_cond @{thm delete_min_on_set} [with_term "tree_set (snd (del_min ?t))"] *}
+setup \<open>add_forward_prfstep_cond @{thm delete_min_on_set} [with_term "tree_set (snd (del_min ?t))"]\<close>
 
 lemma delete_min_interval_inv [forward_arg]:
   "tree_interval_inv t \<Longrightarrow> t \<noteq> Tip \<Longrightarrow> tree_interval_inv (snd (del_min t))" by auto2
@@ -170,7 +170,7 @@ fun delete_elt_tree :: "interval_tree \<Rightarrow> interval_tree" where
          rt' = snd (del_min rt);
          m' = max3 x' (tmax lt) (tmax rt') in
        Node lt (fst (del_min rt)) m' rt')"
-setup {* add_rewrite_rule @{thm delete_elt_tree.simps(2)} *}
+setup \<open>add_rewrite_rule @{thm delete_elt_tree.simps(2)}\<close>
 
 lemma delete_elt_in_traverse [rewrite]:
   "in_traverse (delete_elt_tree (Node lt x m rt)) = in_traverse lt @ in_traverse rt" by auto2
@@ -197,7 +197,7 @@ fun delete :: "nat idx_interval \<Rightarrow> interval_tree \<Rightarrow> interv
      else
        let r' = delete x r;
            m' = max3 y (tmax l) (tmax r') in Node l y m' r')"
-setup {* fold add_rewrite_rule @{thms delete.simps} *}
+setup \<open>fold add_rewrite_rule @{thms delete.simps}\<close>
 
 lemma tree_delete_in_traverse [rewrite]:
   "tree_sorted t \<Longrightarrow> in_traverse (delete x t) = remove_elt_list x (in_traverse t)"
@@ -222,7 +222,7 @@ fun search :: "interval_tree \<Rightarrow> nat interval \<Rightarrow> bool" wher
    (if is_overlap (int y) x then True
     else if l \<noteq> Tip \<and> tmax l \<ge> low x then search l x
     else search r x)"
-setup {* fold add_rewrite_rule @{thms search.simps} *}
+setup \<open>fold add_rewrite_rule @{thms search.simps}\<close>
 
 lemma search_correct [rewrite]:
   "is_interval_tree t \<Longrightarrow> is_interval x \<Longrightarrow> search t x \<longleftrightarrow> has_overlap (tree_set t) x"
