HOL/DataStrs/Mapping_Str.thy
@@ -16,30 +16,30 @@ datatype ('a, 'b) map = Map "'a \<Rightarrow> 'b option"
 
 fun meval :: "('a, 'b) map \<Rightarrow> 'a \<Rightarrow> 'b option" ("_\<langle>_\<rangle>" [90]) where
   "(Map f) \<langle>h\<rangle> = f h"
-setup {* add_rewrite_rule @{thm meval.simps} *}
+setup \<open>add_rewrite_rule @{thm meval.simps}\<close>
 
 lemma meval_ext: "\<forall>x. M\<langle>x\<rangle> = N\<langle>x\<rangle> \<Longrightarrow> M = N"
   apply (cases M) apply (cases N) by auto
-setup {* add_backward_prfstep_cond @{thm meval_ext} [with_filt (order_filter "M" "N")] *}
+setup \<open>add_backward_prfstep_cond @{thm meval_ext} [with_filt (order_filter "M" "N")]\<close>
 
 definition empty_map :: "('a, 'b) map" where
   "empty_map = Map (\<lambda>x. None)"
-setup {* add_rewrite_rule @{thm empty_map_def} *}
+setup \<open>add_rewrite_rule @{thm empty_map_def}\<close>
 
 definition update_map :: "('a, 'b) map \<Rightarrow> 'a \<Rightarrow> 'b \<Rightarrow> ('a ,'b) map" (" _ { _ \<rightarrow> _ }" [89,90,90] 90) where
   "M {k \<rightarrow> v} = Map (\<lambda>x. if x = k then Some v else M\<langle>x\<rangle>)"
-setup {* add_rewrite_rule @{thm update_map_def} *}
+setup \<open>add_rewrite_rule @{thm update_map_def}\<close>
 
 definition delete_map :: "'a \<Rightarrow> ('a, 'b) map \<Rightarrow> ('a, 'b) map" where
   "delete_map k M = Map (\<lambda>x. if x = k then None else M\<langle>x\<rangle>)"
-setup {* add_rewrite_rule @{thm delete_map_def} *}
+setup \<open>add_rewrite_rule @{thm delete_map_def}\<close>
 
 subsection \<open>Map from an AList\<close>
 
 fun map_of_alist :: "('a \<times> 'b) list \<Rightarrow> ('a, 'b) map" where
   "map_of_alist [] = empty_map"
 | "map_of_alist (x # xs) = (map_of_alist xs) {fst x \<rightarrow> snd x}"
-setup {* fold add_rewrite_rule @{thms map_of_alist.simps} *}
+setup \<open>fold add_rewrite_rule @{thms map_of_alist.simps}\<close>
 
 definition has_key_alist :: "('a \<times> 'b) list \<Rightarrow> 'a \<Rightarrow> bool" where [rewrite]:
   "has_key_alist xs a \<longleftrightarrow> (\<exists>p\<in>set xs. fst p = a)"
@@ -47,7 +47,7 @@ definition has_key_alist :: "('a \<times> 'b) list \<Rightarrow> 'a \<Rightarrow
 lemma map_of_alist_nil [rewrite_back]:
   "has_key_alist ys x \<longleftrightarrow> (map_of_alist ys)\<langle>x\<rangle> \<noteq> None"
 @proof @induct ys @qed
-setup {* add_rewrite_rule_cond @{thm map_of_alist_nil} [with_term "(map_of_alist ?ys)\<langle>?x\<rangle>"] *}
+setup \<open>add_rewrite_rule_cond @{thm map_of_alist_nil} [with_term "(map_of_alist ?ys)\<langle>?x\<rangle>"]\<close>
 
 lemma map_of_alist_some [forward]:
   "(map_of_alist xs)\<langle>k\<rangle> = Some v \<Longrightarrow> (k, v) \<in> set xs"
@@ -56,7 +56,7 @@ lemma map_of_alist_some [forward]:
 lemma map_of_alist_nil':
   "x \<in> set (map fst ys) \<longleftrightarrow> (map_of_alist ys)\<langle>x\<rangle> \<noteq> None"
 @proof @induct ys @qed
-setup {* add_rewrite_rule_cond @{thm map_of_alist_nil'} [with_term "(map_of_alist ?ys)\<langle>?x\<rangle>"] *}
+setup \<open>add_rewrite_rule_cond @{thm map_of_alist_nil'} [with_term "(map_of_alist ?ys)\<langle>?x\<rangle>"]\<close>
     
 subsection \<open>Mapping defined by a set of key-value pairs\<close>
 
@@ -64,12 +64,12 @@ definition unique_keys_set :: "('a \<times> 'b) set \<Rightarrow> bool" where [r
   "unique_keys_set S = (\<forall>i x y. (i, x) \<in> S \<longrightarrow> (i, y) \<in> S \<longrightarrow> x = y)"
 
 lemma unique_keys_setD [forward]: "unique_keys_set S \<Longrightarrow> (i, x) \<in> S \<Longrightarrow> (i, y) \<in> S \<Longrightarrow> x = y" by auto2
-setup {* del_prfstep_thm_eqforward @{thm unique_keys_set_def} *}
+setup \<open>del_prfstep_thm_eqforward @{thm unique_keys_set_def}\<close>
 
 definition map_of_aset :: "('a \<times> 'b) set \<Rightarrow> ('a, 'b) map" where
   "map_of_aset S = Map (\<lambda>a. if \<exists>b. (a, b) \<in> S then Some (THE b. (a, b) \<in> S) else None)"
-setup {* add_rewrite_rule @{thm map_of_aset_def} *}
-setup {* add_prfstep_check_req ("map_of_aset S", "unique_keys_set S") *}
+setup \<open>add_rewrite_rule @{thm map_of_aset_def}\<close>
+setup \<open>add_prfstep_check_req ("map_of_aset S", "unique_keys_set S")\<close>
 
 lemma map_of_asetI1 [rewrite]: "unique_keys_set S \<Longrightarrow> (a, b) \<in> S \<Longrightarrow> (map_of_aset S)\<langle>a\<rangle> = Some b"
 @proof @have "\<exists>b. (a, b) \<in> S" @have "\<exists>!b. (a, b) \<in> S" @qed
@@ -80,7 +80,7 @@ lemma map_of_asetD1 [forward]: "(map_of_aset S)\<langle>a\<rangle> = None \<Long
 
 lemma map_of_asetD2 [forward]:
   "unique_keys_set S \<Longrightarrow> (map_of_aset S)\<langle>a\<rangle> = Some b \<Longrightarrow> (a, b) \<in> S" by auto2
-setup {* del_prfstep_thm @{thm map_of_aset_def} *}
+setup \<open>del_prfstep_thm @{thm map_of_aset_def}\<close>
 
 lemma map_of_aset_insert [rewrite]:
   "unique_keys_set (S \<union> {(k, v)}) \<Longrightarrow> map_of_aset (S \<union> {(k, v)}) = (map_of_aset S) {k \<rightarrow> v}"
@@ -133,7 +133,7 @@ definition keys_of :: "('a, 'b) map \<Rightarrow> 'a set" where [rewrite]:
   "keys_of M = {x. M\<langle>x\<rangle> \<noteq> None}"
 
 lemma keys_of_iff [rewrite_bidir]: "x \<in> keys_of M \<longleftrightarrow> M\<langle>x\<rangle> \<noteq> None" by auto2
-setup {* del_prfstep_thm @{thm keys_of_def} *}
+setup \<open>del_prfstep_thm @{thm keys_of_def}\<close>
 
 lemma keys_of_empty [rewrite]: "keys_of empty_map = {}" by auto2
 
@@ -150,7 +150,7 @@ subsection \<open>General construction and update of maps\<close>
 fun map_constr :: "(nat \<Rightarrow> bool) \<Rightarrow> (nat \<Rightarrow> 'a) \<Rightarrow> nat \<Rightarrow> (nat, 'a) map" where
   "map_constr S f 0 = empty_map"
 | "map_constr S f (Suc k) = (let M = map_constr S f k in if S k then M {k \<rightarrow> f k} else M)"
-setup {* fold add_rewrite_rule @{thms map_constr.simps} *}
+setup \<open>fold add_rewrite_rule @{thms map_constr.simps}\<close>
 
 lemma map_constr_eval [rewrite]:
   "map_constr S f n = Map (\<lambda>i. if i < n then if S i then Some (f i) else None else None)"
@@ -166,7 +166,7 @@ fun map_update_all_impl :: "(nat \<Rightarrow> 'a) \<Rightarrow> (nat, 'a) map \
   "map_update_all_impl f M 0 = M"
 | "map_update_all_impl f M (Suc k) =
    (let M' = map_update_all_impl f M k in if k \<in> keys_of M then M' {k \<rightarrow> f k} else M')"
-setup {* fold add_rewrite_rule @{thms map_update_all_impl.simps} *}
+setup \<open>fold add_rewrite_rule @{thms map_update_all_impl.simps}\<close>
 
 lemma map_update_all_impl_ind [rewrite]:
   "map_update_all_impl f M n = Map (\<lambda>i. if i < n then if i \<in> keys_of M then Some (f i) else None else M\<langle>i\<rangle>)"
