HOL/SepLogic/SepAuto.thy
@@ -17,11 +17,11 @@ begin
 subsection \<open>Partial Heaps\<close>
 
 datatype pheap = pHeap (heapOf: heap) (addrOf: "addr set")
-setup {* add_simple_datatype "pheap" *}
+setup \<open>add_simple_datatype "pheap"\<close>
 
 fun in_range :: "(heap \<times> addr set) \<Rightarrow> bool" where
   "in_range (h,as) \<longleftrightarrow> (\<forall>a\<in>as. a < lim h)"
-setup {* add_rewrite_rule @{thm in_range.simps} *}
+setup \<open>add_rewrite_rule @{thm in_range.simps}\<close>
 
 (* Two heaps agree on a set of addresses. *)
 definition relH :: "addr set \<Rightarrow> heap \<Rightarrow> heap \<Rightarrow> bool" where [rewrite]:
@@ -34,7 +34,7 @@ lemma relH_D [forward]:
 lemma relH_D2 [rewrite]:
   "relH as h h' \<Longrightarrow> a \<in> as \<Longrightarrow> refs h t a = refs h' t a"
   "relH as h h' \<Longrightarrow> a \<in> as \<Longrightarrow> arrays h t a = arrays h' t a" by auto2+
-setup {* del_prfstep_thm_eqforward @{thm relH_def} *}
+setup \<open>del_prfstep_thm_eqforward @{thm relH_def}\<close>
 
 lemma relH_dist_union [forward]:
   "relH (as \<union> as') h h' \<Longrightarrow> relH as h h' \<and> relH as' h h'" by auto2
@@ -61,7 +61,7 @@ datatype assn_raw = Assn (assn_fn: "pheap \<Rightarrow> bool")
 
 fun aseval :: "assn_raw \<Rightarrow> pheap \<Rightarrow> bool" where
   "aseval (Assn f) h = f h"
-setup {* add_rewrite_rule @{thm aseval.simps} *}
+setup \<open>add_rewrite_rule @{thm aseval.simps}\<close>
 
 definition proper :: "assn_raw \<Rightarrow> bool" where [rewrite]:
   "proper P = (
@@ -70,14 +70,14 @@ definition proper :: "assn_raw \<Rightarrow> bool" where [rewrite]:
 
 fun in_range_assn :: "pheap \<Rightarrow> bool" where
   "in_range_assn (pHeap h as) \<longleftrightarrow> (\<forall>a\<in>as. a < lim h)"
-setup {* add_rewrite_rule @{thm in_range_assn.simps} *}
+setup \<open>add_rewrite_rule @{thm in_range_assn.simps}\<close>
 
 typedef assn = "Collect proper"
 @proof @have "Assn in_range_assn \<in> Collect proper" @qed
 
-setup {* add_rewrite_rule @{thm Rep_assn_inject} *}
-setup {* register_wellform_data ("Abs_assn P", ["proper P"]) *}
-setup {* add_prfstep_check_req ("Abs_assn P", "proper P") *}
+setup \<open>add_rewrite_rule @{thm Rep_assn_inject}\<close>
+setup \<open>register_wellform_data ("Abs_assn P", ["proper P"])\<close>
+setup \<open>add_prfstep_check_req ("Abs_assn P", "proper P")\<close>
 
 lemma Abs_assn_inverse' [rewrite]: "proper y \<Longrightarrow> Rep_assn (Abs_assn y) = y"
   by (simp add: Abs_assn_inverse)
@@ -99,7 +99,7 @@ instance .. end
 abbreviation one_assn :: assn ("emp") where "one_assn \<equiv> 1"
 
 lemma one_assn_rule [rewrite]: "h \<Turnstile> emp \<longleftrightarrow> addrOf h = {}" by auto2
-setup {* del_prfstep_thm @{thm one_assn_def} *}
+setup \<open>del_prfstep_thm @{thm one_assn_def}\<close>
 
 instantiation assn :: times begin
 definition times_assn where [rewrite]:
@@ -110,16 +110,16 @@ instance .. end
 
 lemma mod_star_conv [rewrite]:
   "pHeap h as \<Turnstile> A * B \<longleftrightarrow> (\<exists>as1 as2. as = as1 \<union> as2 \<and> as1 \<inter> as2 = {} \<and> pHeap h as1 \<Turnstile> A \<and> pHeap h as2 \<Turnstile> B)" by auto2
-setup {* del_prfstep_thm @{thm times_assn_def} *}
+setup \<open>del_prfstep_thm @{thm times_assn_def}\<close>
 
 lemma aseval_ext [backward]: "\<forall>h. aseval P h = aseval P' h \<Longrightarrow> P = P'"
   apply (cases P) apply (cases P') by auto
 
 lemma assn_ext: "\<forall>h as. pHeap h as \<Turnstile> P \<longleftrightarrow> pHeap h as \<Turnstile> Q \<Longrightarrow> P = Q"
 @proof @have "Rep_assn P = Rep_assn Q" @qed
-setup {* add_backward_prfstep_cond @{thm assn_ext} [with_filt (order_filter "P" "Q")] *}
+setup \<open>add_backward_prfstep_cond @{thm assn_ext} [with_filt (order_filter "P" "Q")]\<close>
 
-setup {* del_prfstep_thm @{thm aseval_ext} *}
+setup \<open>del_prfstep_thm @{thm aseval_ext}\<close>
 
 lemma assn_one_left: "1 * P = (P::assn)"
 @proof
@@ -169,7 +169,7 @@ definition ex_assn :: "('a \<Rightarrow> assn) \<Rightarrow> assn" (binder "\<ex
   "(\<exists>\<^sub>Ax. P x) = Abs_assn (Assn (\<lambda>h. \<exists>x. h \<Turnstile> P x))"
 
 lemma mod_ex_dist [rewrite]: "(h \<Turnstile> (\<exists>\<^sub>Ax. P x)) \<longleftrightarrow> (\<exists>x. h \<Turnstile> P x)" by auto2
-setup {* del_prfstep_thm @{thm ex_assn_def} *}
+setup \<open>del_prfstep_thm @{thm ex_assn_def}\<close>
 
 lemma ex_distrib_star: "(\<exists>\<^sub>Ax. P x * Q) = (\<exists>\<^sub>Ax. P x) * Q"
 @proof
@@ -190,7 +190,7 @@ definition sngr_assn :: "'a::heap ref \<Rightarrow> 'a \<Rightarrow> assn" (infi
 
 lemma sngr_assn_rule [rewrite]:
   "pHeap h as \<Turnstile> r \<mapsto>\<^sub>r x \<longleftrightarrow> (Ref.get h r = x \<and> as = {addr_of_ref r} \<and> addr_of_ref r < lim h)" by auto2
-setup {* del_prfstep_thm @{thm sngr_assn_def} *}
+setup \<open>del_prfstep_thm @{thm sngr_assn_def}\<close>
 
 definition snga_assn :: "'a::heap array \<Rightarrow> 'a list \<Rightarrow> assn" (infix "\<mapsto>\<^sub>a" 82) where [rewrite]:
   "r \<mapsto>\<^sub>a x = Abs_assn (Assn (
@@ -198,7 +198,7 @@ definition snga_assn :: "'a::heap array \<Rightarrow> 'a list \<Rightarrow> assn
 
 lemma snga_assn_rule [rewrite]:
   "pHeap h as \<Turnstile> r \<mapsto>\<^sub>a x \<longleftrightarrow> (Array.get h r = x \<and> as = {addr_of_array r} \<and> addr_of_array r < lim h)" by auto2
-setup {* del_prfstep_thm @{thm snga_assn_def} *}
+setup \<open>del_prfstep_thm @{thm snga_assn_def}\<close>
 
 subsubsection \<open>Pure Assertions\<close>
 
@@ -206,15 +206,15 @@ definition pure_assn :: "bool \<Rightarrow> assn" ("\<up>") where [rewrite]:
   "\<up>b = Abs_assn (Assn (\<lambda>h. addrOf h = {} \<and> b))"
 
 lemma pure_assn_rule [rewrite]: "h \<Turnstile> \<up>b \<longleftrightarrow> (addrOf h = {} \<and> b)" by auto2
-setup {* del_prfstep_thm @{thm pure_assn_def} *}
+setup \<open>del_prfstep_thm @{thm pure_assn_def}\<close>
 
 definition top_assn :: assn ("true") where [rewrite]:
   "top_assn = Abs_assn (Assn in_range_assn)"
 
 lemma top_assn_rule [rewrite]: "pHeap h as \<Turnstile> true \<longleftrightarrow> in_range (h, as)" by auto2
-setup {* del_prfstep_thm @{thm top_assn_def} *}
+setup \<open>del_prfstep_thm @{thm top_assn_def}\<close>
 
-setup {* del_prfstep_thm @{thm models_def} *}
+setup \<open>del_prfstep_thm @{thm models_def}\<close>
 
 subsubsection \<open>Properties of assertions\<close>
 
@@ -258,7 +258,7 @@ lemma entails_ex: "\<not>((\<exists>\<^sub>Ax. P x) \<Longrightarrow>\<^sub>A Q)
 lemma entails_ex_post: "\<not>(P \<Longrightarrow>\<^sub>A (\<exists>\<^sub>Ax. Q x)) \<Longrightarrow> \<forall>x. \<not>(P \<Longrightarrow>\<^sub>A Q x)" by auto2
 lemma entails_pure_post: "\<not>(P \<Longrightarrow>\<^sub>A Q * \<up>b) \<Longrightarrow> P \<Longrightarrow>\<^sub>A Q \<Longrightarrow> \<not>b" by auto2
 
-setup {* del_prfstep_thm @{thm entails_def} *}
+setup \<open>del_prfstep_thm @{thm entails_def}\<close>
 
 subsection \<open>Definition of the run predicate\<close>
 
@@ -266,9 +266,9 @@ inductive run :: "'a Heap \<Rightarrow> heap option \<Rightarrow> heap option \<
   "run c None None r"
 | "execute c h = None \<Longrightarrow> run c (Some h) None r"
 | "execute c h = Some (r, h') \<Longrightarrow> run c (Some h) (Some h') r"
-setup {* add_case_induct_rule @{thm run.cases} *}
-setup {* fold add_resolve_prfstep @{thms run.intros(1,2)} *}
-setup {* add_forward_prfstep @{thm run.intros(3)} *}
+setup \<open>add_case_induct_rule @{thm run.cases}\<close>
+setup \<open>fold add_resolve_prfstep @{thms run.intros(1,2)}\<close>
+setup \<open>add_forward_prfstep @{thm run.intros(3)}\<close>
 
 lemma run_complete [resolve]:
   "\<exists>\<sigma>' r. run c \<sigma> \<sigma>' (r::'a)"
@@ -282,13 +282,13 @@ lemma run_to_execute [forward]:
   "run c (Some h) \<sigma>' r \<Longrightarrow> if \<sigma>' = None then execute c h = None else execute c h = Some (r, the \<sigma>')"
 @proof @case_induct "run c (Some h) \<sigma>' r" @qed
 
-setup {* add_rewrite_rule @{thm execute_bind(1)} *}
+setup \<open>add_rewrite_rule @{thm execute_bind(1)}\<close>
 lemma runE [forward]:
   "run f (Some h) (Some h') r' \<Longrightarrow> run (f \<bind> g) (Some h) \<sigma> r \<Longrightarrow> run (g r') (Some h') \<sigma> r" by auto2
 
-setup {* add_rewrite_rule @{thm Array.get_alloc} *}
-setup {* add_rewrite_rule @{thm Ref.get_alloc} *}
-setup {* add_rewrite_rule_bidir @{thm Array.length_def} *}
+setup \<open>add_rewrite_rule @{thm Array.get_alloc}\<close>
+setup \<open>add_rewrite_rule @{thm Ref.get_alloc}\<close>
+setup \<open>add_rewrite_rule_bidir @{thm Array.length_def}\<close>
 
 subsection \<open>Definition of hoare triple, and the frame rule.\<close>
 
@@ -305,7 +305,7 @@ lemma hoare_tripleD [forward]:
      (\<sigma> \<noteq> None \<and> pHeap (the \<sigma>) (new_addrs h as (the \<sigma>)) \<Turnstile> Q r \<and> relH {a . a < lim h \<and> a \<notin> as} h (the \<sigma>) \<and>
      lim h \<le> lim (the \<sigma>))"
   by auto2
-setup {* del_prfstep_thm_eqforward @{thm hoare_triple_def} *}
+setup \<open>del_prfstep_thm_eqforward @{thm hoare_triple_def}\<close>
 
 abbreviation hoare_triple' :: "assn \<Rightarrow> 'r Heap \<Rightarrow> ('r \<Rightarrow> assn) \<Rightarrow> bool" ("<_> _ <_>\<^sub>t") where
   "<P> c <Q>\<^sub>t \<equiv> <P> c <\<lambda>r. Q r * true>"
@@ -323,7 +323,7 @@ lemma frame_rule [backward]:
 @qed
 
 (* This is the last use of the definition of separating conjunction. *)
-setup {* del_prfstep_thm @{thm mod_star_conv} *}
+setup \<open>del_prfstep_thm @{thm mod_star_conv}\<close>
 
 lemma bind_rule:
   "<P> f <Q> \<Longrightarrow> \<forall>x. <Q x> g x <R> \<Longrightarrow> <P> f \<bind> g <R>"
@@ -370,7 +370,7 @@ lemma pre_pure_rule':
 lemma post_rule:
   "<P> f <Q> \<Longrightarrow> \<forall>x. Q x \<Longrightarrow>\<^sub>A R x \<Longrightarrow> <P> f <R>" by auto2
 
-setup {* fold del_prfstep_thm [@{thm entailsD}, @{thm entails_frame}, @{thm frame_rule}] *}
+setup \<open>fold del_prfstep_thm [@{thm entailsD}, @{thm entails_frame}, @{thm frame_rule}]\<close>
 
 (* Actual statement used: *)
 lemma post_rule':
@@ -382,7 +382,7 @@ lemma norm_pre_pure_iff2: "<\<up>b> c <Q> \<longleftrightarrow> (b \<longrightar
 subsection \<open>Hoare triples for atomic commands\<close>
 
 (* First, those that do not modify the heap. *)
-setup {* add_rewrite_rule @{thm execute_assert(1)} *}
+setup \<open>add_rewrite_rule @{thm execute_assert(1)}\<close>
 lemma assert_rule:
   "<\<up>(R x)> assert R x <\<lambda>r. \<up>(r = x)>" by auto2
 
@@ -390,34 +390,34 @@ lemma execute_return' [rewrite]: "execute (return x) h = Some (x, h)" by (metis 
 lemma return_rule:
   "<emp> return x <\<lambda>r. \<up>(r = x)>" by auto2
 
-setup {* add_rewrite_rule @{thm execute_nth(1)} *}
+setup \<open>add_rewrite_rule @{thm execute_nth(1)}\<close>
 lemma nth_rule:
   "<a \<mapsto>\<^sub>a xs * \<up>(i < length xs)> Array.nth a i <\<lambda>r. a \<mapsto>\<^sub>a xs * \<up>(r = xs ! i)>" by auto2
 
-setup {* add_rewrite_rule @{thm execute_len} *}
+setup \<open>add_rewrite_rule @{thm execute_len}\<close>
 lemma length_rule:
   "<a \<mapsto>\<^sub>a xs> Array.len a <\<lambda>r. a \<mapsto>\<^sub>a xs * \<up>(r = length xs)>" by auto2
 
-setup {* add_rewrite_rule @{thm execute_lookup} *}
+setup \<open>add_rewrite_rule @{thm execute_lookup}\<close>
 lemma lookup_rule:
   "<p \<mapsto>\<^sub>r x> !p <\<lambda>r. p \<mapsto>\<^sub>r x * \<up>(r = x)>" by auto2
 
-setup {* add_rewrite_rule @{thm execute_freeze} *}
+setup \<open>add_rewrite_rule @{thm execute_freeze}\<close>
 lemma freeze_rule:
   "<a \<mapsto>\<^sub>a xs> Array.freeze a <\<lambda>r. a \<mapsto>\<^sub>a xs * \<up>(r = xs)>" by auto2
 
 (* Next, the update rules. *)
-setup {* add_rewrite_rule @{thm Ref.lim_set} *}
+setup \<open>add_rewrite_rule @{thm Ref.lim_set}\<close>
 lemma Array_lim_set [rewrite]: "lim (Array.set p xs h) = lim h" by (simp add: Array.set_def)
 
-setup {* fold add_rewrite_rule [@{thm Ref.get_set_eq}, @{thm Array.get_set_eq}] *}
-setup {* add_rewrite_rule @{thm Array.update_def} *}
+setup \<open>fold add_rewrite_rule [@{thm Ref.get_set_eq}, @{thm Array.get_set_eq}]\<close>
+setup \<open>add_rewrite_rule @{thm Array.update_def}\<close>
 
-setup {* add_rewrite_rule @{thm execute_upd(1)} *}
+setup \<open>add_rewrite_rule @{thm execute_upd(1)}\<close>
 lemma upd_rule:
   "<a \<mapsto>\<^sub>a xs * \<up>(i < length xs)> Array.upd i x a <\<lambda>r. a \<mapsto>\<^sub>a list_update xs i x * \<up>(r = a)>" by auto2
 
-setup {* add_rewrite_rule @{thm execute_update} *}
+setup \<open>add_rewrite_rule @{thm execute_update}\<close>
 lemma update_rule:
   "<p \<mapsto>\<^sub>r y> p := x <\<lambda>r. p \<mapsto>\<^sub>r x>" by auto2
 
@@ -428,8 +428,8 @@ lemma Array_alloc_def' [rewrite]:
   "Array.alloc xs h = (let l = lim h; r = Array l in (r, (Array.set r xs (h\<lparr>lim := l + 1\<rparr>))))"
   by (simp add: Array.alloc_def)
 
-setup {* fold add_rewrite_rule [
-  @{thm addr_of_array.simps}, @{thm addr_of_ref.simps}, @{thm Ref.alloc_def}] *}
+setup \<open>fold add_rewrite_rule [
+  @{thm addr_of_array.simps}, @{thm addr_of_ref.simps}, @{thm Ref.alloc_def}]\<close>
 
 lemma refs_on_Array_set [rewrite]: "refs (Array.set p xs h) t i = refs h t i"
   by (simp add: Array.set_def)
@@ -451,22 +451,22 @@ lemma refs_on_Ref_alloc [rewrite]: "i < lim h \<Longrightarrow> refs (snd (Ref.a
   by (smt Ref.alloc_def Ref.set_def addr_of_ref.simps fun_upd_apply less_or_eq_imp_le
           linorder_not_less select_convs(2) simps(6) snd_conv surjective update_convs(3))
 
-setup {* add_rewrite_rule @{thm execute_new} *}
+setup \<open>add_rewrite_rule @{thm execute_new}\<close>
 lemma new_rule:
   "<emp> Array.new n x <\<lambda>r. r \<mapsto>\<^sub>a replicate n x>" by auto2
 
-setup {* add_rewrite_rule @{thm execute_of_list} *}
+setup \<open>add_rewrite_rule @{thm execute_of_list}\<close>
 lemma of_list_rule:
   "<emp> Array.of_list xs <\<lambda>r. r \<mapsto>\<^sub>a xs>" by auto2
 
-setup {* add_rewrite_rule @{thm execute_ref} *}
+setup \<open>add_rewrite_rule @{thm execute_ref}\<close>
 lemma ref_rule:
   "<emp> ref x <\<lambda>r. r \<mapsto>\<^sub>r x>" by auto2
 
-setup {* fold del_prfstep_thm [
+setup \<open>fold del_prfstep_thm [
   @{thm sngr_assn_rule}, @{thm snga_assn_rule}, @{thm pure_assn_rule}, @{thm top_assn_rule},
-  @{thm mod_pure_star_dist}, @{thm one_assn_rule}, @{thm hoare_triple_def}, @{thm mod_ex_dist}] *}
-setup {* del_simple_datatype "pheap" *}
+  @{thm mod_pure_star_dist}, @{thm one_assn_rule}, @{thm hoare_triple_def}, @{thm mod_ex_dist}]\<close>
+setup \<open>del_simple_datatype "pheap"\<close>
 
 subsection \<open>Definition of procedures\<close>
 
@@ -479,7 +479,7 @@ abbreviation (input) models_ascii :: "pheap \<Rightarrow> assn \<Rightarrow> boo
 
 ML_file "sep_util.ML"
 
-ML {*
+ML \<open>
 structure AssnMatcher = AssnMatcher(SepUtil)
 structure SepLogic = SepLogic(SepUtil)
 val add_assn_matcher = AssnMatcher.add_assn_matcher
@@ -487,20 +487,20 @@ val add_entail_matcher = AssnMatcher.add_entail_matcher
 val add_forward_ent_prfstep = SepLogic.add_forward_ent_prfstep
 val add_rewrite_ent_rule = SepLogic.add_rewrite_ent_rule
 val add_hoare_triple_prfstep = SepLogic.add_hoare_triple_prfstep
-*}
-setup {* AssnMatcher.add_assn_matcher_proofsteps *}
-setup {* SepLogic.add_sep_logic_proofsteps *}
+\<close>
+setup \<open>AssnMatcher.add_assn_matcher_proofsteps\<close>
+setup \<open>SepLogic.add_sep_logic_proofsteps\<close>
 
 ML_file "sep_steps_test.ML"
 
-attribute_setup forward_ent = {* setup_attrib add_forward_ent_prfstep *}
-attribute_setup rewrite_ent = {* setup_attrib add_rewrite_ent_rule *}
-attribute_setup hoare_triple = {* setup_attrib add_hoare_triple_prfstep *}
+attribute_setup forward_ent = \<open>setup_attrib add_forward_ent_prfstep\<close>
+attribute_setup rewrite_ent = \<open>setup_attrib add_rewrite_ent_rule\<close>
+attribute_setup hoare_triple = \<open>setup_attrib add_hoare_triple_prfstep\<close>
 
-setup {* fold add_hoare_triple_prfstep [
+setup \<open>fold add_hoare_triple_prfstep [
   @{thm assert_rule}, @{thm update_rule}, @{thm nth_rule}, @{thm upd_rule},
   @{thm return_rule}, @{thm ref_rule}, @{thm lookup_rule}, @{thm new_rule},
-  @{thm of_list_rule}, @{thm length_rule}, @{thm freeze_rule}] *}
+  @{thm of_list_rule}, @{thm length_rule}, @{thm freeze_rule}]\<close>
 
 (* Some simple tests *)
 
