HOL/Arith_Thms.thy
@@ -63,7 +63,7 @@ ML_file "order.ML"
 ML_file "order_test.ML"
 
 setup \<open>register_wellform_data ("(a::nat) - b", ["a \<ge> b"])\<close>
-setup {* add_prfstep_check_req ("(a::nat) - b", "(a::nat) \<ge> b") *}
+setup \<open>add_prfstep_check_req ("(a::nat) - b", "(a::nat) \<ge> b")\<close>
 
 (* Normalize any expression to "a - b" form. *)
 lemma nat_sub_norm:
@@ -99,52 +99,52 @@ ML_file "nat_sub_test.ML"
 lemma le_neq_implies_less' [forward]: "(m::nat) \<noteq> n \<Longrightarrow> m \<le> n \<Longrightarrow> m < n" by simp
 lemma le_zero_to_equal_zero [forward]: "(n::nat) \<le> 0 \<Longrightarrow> n = 0" by simp
 lemma less_one_to_equal_zero [forward]: "(n::nat) < 1 \<Longrightarrow> n = 0" by simp
-setup {* add_backward_prfstep_cond @{thm Nat.mult_le_mono1} [with_cond "?k \<noteq> 1"] *}
-setup {* add_resolve_prfstep @{thm Nat.not_add_less1} *}
+setup \<open>add_backward_prfstep_cond @{thm Nat.mult_le_mono1} [with_cond "?k \<noteq> 1"]\<close>
+setup \<open>add_resolve_prfstep @{thm Nat.not_add_less1}\<close>
 lemma not_minus_less [resolve]: "\<not>(i::nat) < (i - j)" by simp
 lemma nat_le_prod_with_same [backward]: "m \<noteq> 0 \<Longrightarrow> (n::nat) \<le> m * n" by simp
 lemma nat_le_prod_with_le [backward1]: "k \<noteq> 0 \<Longrightarrow> (n::nat) \<le> m \<Longrightarrow> (n::nat) \<le> k * m"
   using le_trans nat_le_prod_with_same by blast
 lemma nat_plus_le_to_less [backward1]: "b \<noteq> 0 \<Longrightarrow> (a::nat) + b \<le> c \<Longrightarrow> a < c" by simp
 lemma nat_plus_le_to_less2 [backward1]: "a \<noteq> 0 \<Longrightarrow> (a::nat) + b \<le> c \<Longrightarrow> b < c" by simp
-setup {* add_forward_prfstep @{thm add_right_imp_eq} *}
-setup {* add_forward_prfstep @{thm add_left_imp_eq} *}
+setup \<open>add_forward_prfstep @{thm add_right_imp_eq}\<close>
+setup \<open>add_forward_prfstep @{thm add_left_imp_eq}\<close>
 
-setup {* add_rewrite_rule_cond @{thm Nat.le_diff_conv2} [with_term "?i + ?k"] *}
+setup \<open>add_rewrite_rule_cond @{thm Nat.le_diff_conv2} [with_term "?i + ?k"]\<close>
 lemma nat_less_diff_conv: "(i::nat) < j - k \<Longrightarrow> i + k < j" by simp
-setup {* add_forward_prfstep_cond @{thm nat_less_diff_conv} [with_cond "?k \<noteq> ?NUMC", with_term "?i + ?k"]*}
+setup \<open>add_forward_prfstep_cond @{thm nat_less_diff_conv} [with_cond "?k \<noteq> ?NUMC", with_term "?i + ?k"]\<close>
 lemma Nat_le_diff_conv2_same [forward]: "i \<ge> j \<Longrightarrow> (i::nat) \<le> i - j \<Longrightarrow> j = 0" by simp
 lemma nat_gt_zero [forward]: "b - a > 0 \<Longrightarrow> b > (a::nat)" by simp
 lemma n_minus_1_less_n: "(n::nat) \<ge> 1 \<Longrightarrow> n - 1 < n" by simp
-setup {* add_forward_prfstep_cond @{thm n_minus_1_less_n} [with_term "?n - 1"] *}
+setup \<open>add_forward_prfstep_cond @{thm n_minus_1_less_n} [with_term "?n - 1"]\<close>
   
 (* Monotonicity of ordering *)
-setup {* add_backward_prfstep @{thm Nat.diff_le_mono} *}
-setup {* add_backward2_prfstep @{thm Nat.diff_less_mono} *}
-setup {* add_backward_prfstep @{thm Nat.mult_le_mono2} *}
-setup {* add_resolve_prfstep @{thm Nat.le_add1} *}
-setup {* add_resolve_prfstep @{thm Nat.le_add2} *}
-setup {* add_backward_prfstep @{thm add_left_mono} *}
-setup {* add_backward_prfstep @{thm add_right_mono} *}
+setup \<open>add_backward_prfstep @{thm Nat.diff_le_mono}\<close>
+setup \<open>add_backward2_prfstep @{thm Nat.diff_less_mono}\<close>
+setup \<open>add_backward_prfstep @{thm Nat.mult_le_mono2}\<close>
+setup \<open>add_resolve_prfstep @{thm Nat.le_add1}\<close>
+setup \<open>add_resolve_prfstep @{thm Nat.le_add2}\<close>
+setup \<open>add_backward_prfstep @{thm add_left_mono}\<close>
+setup \<open>add_backward_prfstep @{thm add_right_mono}\<close>
 lemma add_mono_neutr [backward]: "(0::'a::linordered_ring) \<le> b \<Longrightarrow> a \<le> a + b" by simp
 lemma add_mono_neutl [backward]: "(0::'a::linordered_ring) \<le> b \<Longrightarrow> a \<le> b + a" by simp
-setup {* add_forward_prfstep @{thm add_less_imp_less_left} *}
+setup \<open>add_forward_prfstep @{thm add_less_imp_less_left}\<close>
 lemma sum_le_zero1 [forward]: "(a::'a::linordered_ring) + b < 0 \<Longrightarrow> a \<ge> 0 \<Longrightarrow> b < 0" by (meson add_less_same_cancel1 less_le_trans)
 lemma less_sum1 [backward]: "b > 0 \<Longrightarrow> a < a + (b::nat)" by auto
-setup {* add_backward_prfstep @{thm Nat.trans_less_add2} *}
-setup {* add_backward_prfstep @{thm Nat.add_less_mono1} *}
-setup {* add_backward1_prfstep @{thm Nat.add_less_mono} *}
-setup {* add_backward1_prfstep @{thm Nat.add_le_mono} *}
-setup {* add_backward1_prfstep @{thm add_increasing2} *}
-setup {* add_backward1_prfstep @{thm add_mono} *}
-setup {* add_backward_prfstep @{thm add_strict_left_mono} *}
-setup {* add_backward1_prfstep @{thm Nat.mult_le_mono} *}
+setup \<open>add_backward_prfstep @{thm Nat.trans_less_add2}\<close>
+setup \<open>add_backward_prfstep @{thm Nat.add_less_mono1}\<close>
+setup \<open>add_backward1_prfstep @{thm Nat.add_less_mono}\<close>
+setup \<open>add_backward1_prfstep @{thm Nat.add_le_mono}\<close>
+setup \<open>add_backward1_prfstep @{thm add_increasing2}\<close>
+setup \<open>add_backward1_prfstep @{thm add_mono}\<close>
+setup \<open>add_backward_prfstep @{thm add_strict_left_mono}\<close>
+setup \<open>add_backward1_prfstep @{thm Nat.mult_le_mono}\<close>
 
 (* Addition. *)
 theorem nat_add_eq_self_zero [forward]: "(m::nat) = m + n \<Longrightarrow> n = 0" by simp
 theorem nat_add_eq_self_zero' [forward]: "(m::nat) = n + m \<Longrightarrow> n = 0" by simp
 theorem nat_mult_2: "(a::nat) + a = 2 * a" by simp
-setup {* add_rewrite_rule_cond @{thm nat_mult_2} [with_cond "?a \<noteq> 0"] *}
+setup \<open>add_rewrite_rule_cond @{thm nat_mult_2} [with_cond "?a \<noteq> 0"]\<close>
 theorem plus_one_non_zero [resolve]: "\<not>(n::nat) + 1 = 0" by simp
 
 (* Diff. *)
@@ -155,34 +155,34 @@ lemma diff_eq_zero' [forward]: "(k::nat) \<le> j \<Longrightarrow> j - k + i = j
 (* Divides. *)
 theorem dvd_defD1 [resolve]: "(a::nat) dvd b \<Longrightarrow> \<exists>k. b = a * k" using dvdE by blast
 theorem dvd_defD2 [resolve]: "(a::nat) dvd b \<Longrightarrow> \<exists>k. b = k * a" by (metis dvd_mult_div_cancel mult.commute)
-setup {* add_forward_prfstep @{thm Nat.dvd_imp_le} *}
+setup \<open>add_forward_prfstep @{thm Nat.dvd_imp_le}\<close>
 theorem dvd_ineq2 [forward]: "(k::nat) dvd n \<Longrightarrow> n > 0 \<Longrightarrow> k \<ge> 1" by (simp add: Suc_leI dvd_pos_nat)
 
-setup {* add_forward_prfstep_cond @{thm dvd_trans} (with_conds ["?a \<noteq> ?b", "?b \<noteq> ?c", "?a \<noteq> ?c"]) *}
-setup {* add_forward_prfstep_cond @{thm Nat.dvd_antisym} [with_cond "?m \<noteq> ?n"] *}
+setup \<open>add_forward_prfstep_cond @{thm dvd_trans} (with_conds ["?a \<noteq> ?b", "?b \<noteq> ?c", "?a \<noteq> ?c"])\<close>
+setup \<open>add_forward_prfstep_cond @{thm Nat.dvd_antisym} [with_cond "?m \<noteq> ?n"]\<close>
 theorem dvd_cancel [backward1]: "c > 0 \<Longrightarrow> (a::nat) * c dvd b * c \<Longrightarrow> a dvd b" by simp
-setup {* add_forward_prfstep (equiv_forward_th @{thm dvd_add_right_iff}) *}
+setup \<open>add_forward_prfstep (equiv_forward_th @{thm dvd_add_right_iff})\<close>
 
 (* Divisibility: existence. *)
-setup {* add_resolve_prfstep @{thm dvd_refl} *}
+setup \<open>add_resolve_prfstep @{thm dvd_refl}\<close>
 theorem exists_n_dvd_n [backward]: "P (n::nat) \<Longrightarrow> \<exists>k. k dvd n \<and> P k" using dvd_refl by blast
-setup {* add_resolve_prfstep @{thm one_dvd} *}
+setup \<open>add_resolve_prfstep @{thm one_dvd}\<close>
 
 theorem any_n_dvd_0 [forward]: "\<not> (\<exists> k. k dvd (0::nat) \<and> P k) \<Longrightarrow> \<not> (\<exists> k. P k)" by simp
 
 theorem n_dvd_one: "(n::nat) dvd 1 \<Longrightarrow> n = 1" by simp
-setup {* add_forward_prfstep_cond @{thm n_dvd_one} [with_cond "?n \<noteq> 1"] *}
+setup \<open>add_forward_prfstep_cond @{thm n_dvd_one} [with_cond "?n \<noteq> 1"]\<close>
 
 (* Products. *)
-setup {* add_rewrite_rule @{thm mult_zero_left} *}
+setup \<open>add_rewrite_rule @{thm mult_zero_left}\<close>
 lemma prod_ineqs1 [forward]: "(m::nat) * k > 0 \<Longrightarrow> m > 0 \<and> k > 0" by simp
 lemma prod_ineqs2 [backward]: "(k::nat) > 0 \<Longrightarrow> m \<le> m * k" by simp
 
 theorem prod_cancel: "(a::nat) * b = a * c \<Longrightarrow> a > 0 \<Longrightarrow> b = c" by auto
-setup {* add_forward_prfstep_cond @{thm prod_cancel} [with_cond "?b \<noteq> ?c"] *}
+setup \<open>add_forward_prfstep_cond @{thm prod_cancel} [with_cond "?b \<noteq> ?c"]\<close>
 
 theorem mult_n1n: "(n::nat) = m * n \<Longrightarrow> n > 0 \<Longrightarrow> m = 1" by auto
-setup {* add_forward_prfstep_cond @{thm mult_n1n} [with_cond "?m \<noteq> 1"] *}
+setup \<open>add_forward_prfstep_cond @{thm mult_n1n} [with_cond "?m \<noteq> 1"]\<close>
 
 theorem prod_is_one [forward]: "(x::nat) * y = 1 \<Longrightarrow> x = 1" by simp
 
@@ -190,14 +190,14 @@ theorem prod_dvd_intro [backward]: "(k::nat) dvd m \<or> k dvd n \<Longrightarro
   using dvd_mult dvd_mult2 by blast
 
 (* Definition of gcd. *)
-setup {* add_forward_prfstep_cond @{thm gcd_dvd1} [with_term "gcd ?a ?b"] *}
-setup {* add_forward_prfstep_cond @{thm gcd_dvd2} [with_term "gcd ?a ?b"] *}
+setup \<open>add_forward_prfstep_cond @{thm gcd_dvd1} [with_term "gcd ?a ?b"]\<close>
+setup \<open>add_forward_prfstep_cond @{thm gcd_dvd2} [with_term "gcd ?a ?b"]\<close>
 
 (* Coprimality. *)
-setup {* add_rewrite_rule_bidir @{thm coprime_iff_gcd_eq_1} *}
+setup \<open>add_rewrite_rule_bidir @{thm coprime_iff_gcd_eq_1}\<close>
 lemma coprime_exp [backward]: "coprime d a \<Longrightarrow> coprime (d::nat) (a ^ n)" by simp
-setup {* add_backward_prfstep @{thm coprime_exp} *}
-setup {* add_rewrite_rule @{thm gcd.commute} *}
+setup \<open>add_backward_prfstep @{thm coprime_exp}\<close>
+setup \<open>add_rewrite_rule @{thm gcd.commute}\<close>
 lemma coprime_dvd_mult [backward1]: "coprime (a::nat) b \<Longrightarrow> a dvd c * b \<Longrightarrow> a dvd c"
   by (metis coprime_dvd_mult_left_iff)
 lemma coprime_dvd_mult' [backward1]: "coprime (a::nat) b \<Longrightarrow> a dvd b * c \<Longrightarrow> a dvd c"
@@ -208,34 +208,34 @@ theorem coprime_dvd [forward]:
   using coprime_common_divisor_nat by blast
 
 (* Powers. *)
-setup {* add_rewrite_rule @{thm power_0} *}
+setup \<open>add_rewrite_rule @{thm power_0}\<close>
 theorem power_ge_0 [rewrite]: "m \<noteq> 0 \<Longrightarrow> p ^ m = p * (p ^ (m - 1))" by (simp add: power_eq_if)
-setup {* add_rewrite_rule_cond @{thm power_one} [with_cond "?n \<noteq> 0"] *}
-setup {* add_rewrite_rule_cond @{thm power_one_right} [with_cond "?a \<noteq> 1"] *}
-setup {* add_gen_prfstep ("power_case_intro",
-  [WithTerm @{term_pat "?p ^ (?FREE::nat)"}, CreateCase @{term_pat "(?FREE::nat) = 0"}]) *}
+setup \<open>add_rewrite_rule_cond @{thm power_one} [with_cond "?n \<noteq> 0"]\<close>
+setup \<open>add_rewrite_rule_cond @{thm power_one_right} [with_cond "?a \<noteq> 1"]\<close>
+setup \<open>add_gen_prfstep ("power_case_intro",
+  [WithTerm @{term_pat "?p ^ (?FREE::nat)"}, CreateCase @{term_pat "(?FREE::nat) = 0"}])\<close>
 
 lemma one_is_power_of_any [resolve]: "\<exists>i. (1::nat) = a ^ i" by (metis power.simps(1))
 
-setup {* add_rewrite_rule @{thm power_Suc} *}
+setup \<open>add_rewrite_rule @{thm power_Suc}\<close>
 
 theorem power_dvd [forward]: "(p::nat)^n dvd a \<Longrightarrow> n \<noteq> 0 \<Longrightarrow> p dvd a" using dvd_power dvd_trans by blast
 
 theorem power_eq_one: "(b::nat) ^ n = 1 \<Longrightarrow> b = 1 \<or> n = 0"
   by (metis One_nat_def Suc_lessI nat_zero_less_power_iff power_0 power_inject_exp)
-setup {* add_forward_prfstep_cond @{thm power_eq_one} (with_conds ["?b \<noteq> 1", "?n \<noteq> 0"]) *}
+setup \<open>add_forward_prfstep_cond @{thm power_eq_one} (with_conds ["?b \<noteq> 1", "?n \<noteq> 0"])\<close>
 
 (* Factorial. *)
 theorem fact_ge_1_nat: "fact (n::nat) \<ge> (1::nat)" by simp
-setup {* add_forward_prfstep_cond @{thm fact_ge_1_nat} [with_term "fact ?n"] *}
-setup {* add_backward1_prfstep @{thm dvd_fact} *}
+setup \<open>add_forward_prfstep_cond @{thm fact_ge_1_nat} [with_term "fact ?n"]\<close>
+setup \<open>add_backward1_prfstep @{thm dvd_fact}\<close>
 
 (* Successor function. *)
-setup {* add_rewrite_rule @{thm Nat.Suc_eq_plus1} *}
-setup {* add_backward_prfstep @{thm Nat.gr0_implies_Suc} *}
+setup \<open>add_rewrite_rule @{thm Nat.Suc_eq_plus1}\<close>
+setup \<open>add_backward_prfstep @{thm Nat.gr0_implies_Suc}\<close>
 
 (* Cases *)
-setup {* fold add_rewrite_rule @{thms Nat.nat.case} *}
+setup \<open>fold add_rewrite_rule @{thms Nat.nat.case}\<close>
 
 (* Induction. *)
 lemma nat_cases: "P 0 \<Longrightarrow> (\<And>n. P (Suc n)) \<Longrightarrow> P n" using nat_induct by auto
@@ -243,10 +243,10 @@ lemma nat_cases: "P 0 \<Longrightarrow> (\<And>n. P (Suc n)) \<Longrightarrow> P
 (* div *)
 declare times_div_less_eq_dividend [resolve]
 
-setup {*
+setup \<open>
   add_var_induct_rule @{thm nat_induct} #>
   add_strong_induct_rule @{thm nat_less_induct} #>
   add_cases_rule @{thm nat_cases}
-*}
+\<close>
 
 end
