HOL/Lists_Thms.thy
@@ -13,15 +13,15 @@ begin
 
 subsection \<open>Definition of lists\<close>
 
-setup {* add_resolve_prfstep @{thm list.distinct(2)} *}
-setup {* add_forward_prfstep (equiv_forward_th @{thm list.simps(1)}) *}
-setup {* fold add_rewrite_rule @{thms List.list.sel} *}
-setup {* add_rewrite_rule @{thm list.collapse} *}
-setup {* add_var_induct_rule @{thm list.induct} *}
+setup \<open>add_resolve_prfstep @{thm list.distinct(2)}\<close>
+setup \<open>add_forward_prfstep (equiv_forward_th @{thm list.simps(1)})\<close>
+setup \<open>fold add_rewrite_rule @{thms List.list.sel}\<close>
+setup \<open>add_rewrite_rule @{thm list.collapse}\<close>
+setup \<open>add_var_induct_rule @{thm list.induct}\<close>
 
 subsection \<open>Length\<close>
 
-setup {* add_rewrite_rule @{thm List.list.size(3)} *}
+setup \<open>add_rewrite_rule @{thm List.list.size(3)}\<close>
 lemma length_one [rewrite]: "length [x] = 1" by simp
 lemma length_Cons [rewrite]: "length (a # b) = length b + 1" by simp
 lemma length_snoc [rewrite]: "length (xs @ [x]) = length xs + 1" by auto
@@ -30,9 +30,9 @@ lemma length_gt_zero [forward]: "length xs > 0 \<Longrightarrow> xs \<noteq> []"
 
 subsection \<open>Append\<close>
 
-setup {* add_rewrite_rule @{thm List.length_append} *}
-setup {* add_rewrite_rule_cond @{thm List.append.simps(2)} [with_cond "?xs \<noteq> []"] *}
-setup {* add_rewrite_rule @{thm List.hd_append2} *}
+setup \<open>add_rewrite_rule @{thm List.length_append}\<close>
+setup \<open>add_rewrite_rule_cond @{thm List.append.simps(2)} [with_cond "?xs \<noteq> []"]\<close>
+setup \<open>add_rewrite_rule @{thm List.hd_append2}\<close>
 lemma append_is_empty [forward]: "xs @ ys = [] \<Longrightarrow> xs = [] \<and> ys = []" by simp
 
 lemma cons_to_append [rewrite_back]: "a # b = [a] @ b" by simp
@@ -42,28 +42,28 @@ ML_file "list_ac_test.ML"
 
 subsection \<open>Showing two lists are equal\<close>
 
-setup {* add_backward2_prfstep_cond @{thm nth_equalityI} [with_filt (order_filter "xs" "ys")] *}
+setup \<open>add_backward2_prfstep_cond @{thm nth_equalityI} [with_filt (order_filter "xs" "ys")]\<close>
 
 subsection \<open>Set of elements of a list\<close>
 
-setup {* add_rewrite_rule @{thm List.set_simps(1)} *}
+setup \<open>add_rewrite_rule @{thm List.set_simps(1)}\<close>
 lemma set_one [rewrite]: "set [u] = {u}" by simp
 lemma set_two [rewrite]: "set [u, v] = {u, v}" by simp
 lemma set_simps2: "set (x # xs) = {x} \<union> set xs" by simp
-setup {* add_rewrite_rule_cond @{thm set_simps2} [with_cond "?xs \<noteq> []", with_cond "?xs \<noteq> [?y]"] *}
-setup {* add_rewrite_rule @{thm List.set_append} *}
-setup {* add_rewrite_rule @{thm List.set_rev} *}
-setup {* add_resolve_prfstep @{thm List.finite_set} *}
-setup {* add_backward_prfstep (equiv_forward_th @{thm in_set_conv_nth}) *}
+setup \<open>add_rewrite_rule_cond @{thm set_simps2} [with_cond "?xs \<noteq> []", with_cond "?xs \<noteq> [?y]"]\<close>
+setup \<open>add_rewrite_rule @{thm List.set_append}\<close>
+setup \<open>add_rewrite_rule @{thm List.set_rev}\<close>
+setup \<open>add_resolve_prfstep @{thm List.finite_set}\<close>
+setup \<open>add_backward_prfstep (equiv_forward_th @{thm in_set_conv_nth})\<close>
 
 subsection \<open>hd\<close>
 
-setup {* register_wellform_data ("hd xs", ["xs \<noteq> []"]) *}
-setup {* add_forward_prfstep_cond @{thm List.hd_in_set} [with_term "hd ?xs"] *}
+setup \<open>register_wellform_data ("hd xs", ["xs \<noteq> []"])\<close>
+setup \<open>add_forward_prfstep_cond @{thm List.hd_in_set} [with_term "hd ?xs"]\<close>
 
 subsection \<open>tl\<close>
 
-setup {* add_rewrite_rule @{thm length_tl} *}
+setup \<open>add_rewrite_rule @{thm length_tl}\<close>
 lemma nth_tl' [rewrite]: "i < length (tl xs) \<Longrightarrow> tl xs ! i = xs ! (i + 1)"
   by (simp add: nth_tl)
 lemma set_tl_subset [forward_arg1]: "set (tl xs) \<subseteq> set xs"
@@ -71,18 +71,18 @@ lemma set_tl_subset [forward_arg1]: "set (tl xs) \<subseteq> set xs"
 
 subsection \<open>nth\<close>
 
-setup {* register_wellform_data ("xs ! i", ["i < length xs"]) *}
-setup {* add_prfstep_check_req ("xs ! i", "i < length xs") *}
-setup {* add_rewrite_rule_back @{thm hd_conv_nth} *}
-setup {* add_rewrite_rule @{thm List.nth_Cons'} *}
-setup {* add_rewrite_rule @{thm List.nth_append} *}
-setup {* add_forward_prfstep_cond @{thm nth_mem} [with_term "?xs ! ?n"] *}
+setup \<open>register_wellform_data ("xs ! i", ["i < length xs"])\<close>
+setup \<open>add_prfstep_check_req ("xs ! i", "i < length xs")\<close>
+setup \<open>add_rewrite_rule_back @{thm hd_conv_nth}\<close>
+setup \<open>add_rewrite_rule @{thm List.nth_Cons'}\<close>
+setup \<open>add_rewrite_rule @{thm List.nth_append}\<close>
+setup \<open>add_forward_prfstep_cond @{thm nth_mem} [with_term "?xs ! ?n"]\<close>
 
 subsection \<open>sorted\<close>
 
 lemma sorted_Nil [resolve]: "sorted []" by simp
 lemma sorted_single [resolve]: "sorted [x]" by simp
-setup {* add_backward_prfstep (equiv_backward_th @{thm sorted.simps(2)}) *}
+setup \<open>add_backward_prfstep (equiv_backward_th @{thm sorted.simps(2)})\<close>
 
 lemma sorted_ConsD1 [forward]: "sorted (x # xs) \<Longrightarrow> sorted xs"
   using sorted.simps(2) by blast
@@ -108,23 +108,23 @@ lemma sorted_nth_mono_less [forward]:
 
 subsection \<open>sort\<close>
 
-setup {* add_forward_prfstep_cond @{thm sorted_sort} [with_term "sort ?xs"] *}
-setup {* add_rewrite_rule @{thm length_sort} *}
-setup {* add_rewrite_rule @{thm mset_sort} *}
-setup {* add_rewrite_rule @{thm set_sort} *}
-setup {* add_backward_prfstep @{thm properties_for_sort} *}
+setup \<open>add_forward_prfstep_cond @{thm sorted_sort} [with_term "sort ?xs"]\<close>
+setup \<open>add_rewrite_rule @{thm length_sort}\<close>
+setup \<open>add_rewrite_rule @{thm mset_sort}\<close>
+setup \<open>add_rewrite_rule @{thm set_sort}\<close>
+setup \<open>add_backward_prfstep @{thm properties_for_sort}\<close>
 lemma sort_Nil [rewrite]: "sort [] = []" by auto
 lemma sort_singleton [rewrite]: "sort [a] = [a]" by auto
 
 subsection \<open>distinct\<close>
   
 lemma distinct_Nil [resolve]: "distinct []" by simp
-setup {* add_resolve_prfstep @{thm List.distinct_singleton} *}
-setup {* add_rewrite_rule_cond @{thm distinct.simps(2)} [with_cond "?xs \<noteq> []"] *}
-setup {* add_rewrite_rule @{thm distinct_append} *}
-setup {* add_rewrite_rule @{thm distinct_rev} *}
-setup {* add_rewrite_rule @{thm distinct_sort} *}
-setup {* add_resolve_prfstep (equiv_backward_th @{thm distinct_conv_nth}) *}
+setup \<open>add_resolve_prfstep @{thm List.distinct_singleton}\<close>
+setup \<open>add_rewrite_rule_cond @{thm distinct.simps(2)} [with_cond "?xs \<noteq> []"]\<close>
+setup \<open>add_rewrite_rule @{thm distinct_append}\<close>
+setup \<open>add_rewrite_rule @{thm distinct_rev}\<close>
+setup \<open>add_rewrite_rule @{thm distinct_sort}\<close>
+setup \<open>add_resolve_prfstep (equiv_backward_th @{thm distinct_conv_nth})\<close>
 
 lemma distinct_nthE [forward]:
   "distinct xs \<Longrightarrow> i < length xs \<Longrightarrow> j < length xs \<Longrightarrow> xs ! i = xs ! j \<Longrightarrow> i = j"
@@ -132,119 +132,119 @@ lemma distinct_nthE [forward]:
 
 subsection \<open>map function\<close>
 
-setup {* fold add_rewrite_rule @{thms List.list.map} *}
-setup {* add_rewrite_rule @{thm List.length_map} *}
-setup {* add_rewrite_rule @{thm List.nth_map} *}
-setup {* add_rewrite_rule @{thm List.map_append} *}
+setup \<open>fold add_rewrite_rule @{thms List.list.map}\<close>
+setup \<open>add_rewrite_rule @{thm List.length_map}\<close>
+setup \<open>add_rewrite_rule @{thm List.nth_map}\<close>
+setup \<open>add_rewrite_rule @{thm List.map_append}\<close>
 
 subsection \<open>Replicate\<close>
 
-setup {* add_rewrite_arg_rule @{thm length_replicate} *}
-setup {* add_rewrite_rule @{thm List.nth_replicate} *}
+setup \<open>add_rewrite_arg_rule @{thm length_replicate}\<close>
+setup \<open>add_rewrite_rule @{thm List.nth_replicate}\<close>
 
 subsection \<open>last\<close>
 
-setup {* register_wellform_data ("last xs", ["xs \<noteq> []"]) *}
+setup \<open>register_wellform_data ("last xs", ["xs \<noteq> []"])\<close>
 lemma last_eval1 [rewrite]: "last [x] = x" by simp
 lemma last_eval2 [rewrite]: "last [u, v] = v" by simp
-setup {* add_rewrite_rule @{thm List.last_ConsR} *}
-setup {* add_rewrite_rule @{thm List.last_appendR} *}
-setup {* add_rewrite_rule @{thm List.last_snoc} *}
-setup {* add_rewrite_rule_back @{thm last_conv_nth} *}
-setup {* add_forward_prfstep_cond @{thm List.last_in_set} [with_term "last ?as"] *}
+setup \<open>add_rewrite_rule @{thm List.last_ConsR}\<close>
+setup \<open>add_rewrite_rule @{thm List.last_appendR}\<close>
+setup \<open>add_rewrite_rule @{thm List.last_snoc}\<close>
+setup \<open>add_rewrite_rule_back @{thm last_conv_nth}\<close>
+setup \<open>add_forward_prfstep_cond @{thm List.last_in_set} [with_term "last ?as"]\<close>
 
 subsection \<open>butlast\<close>
 
-setup {* add_rewrite_arg_rule @{thm List.length_butlast} *}
-setup {* add_rewrite_rule @{thm List.nth_butlast} *}
-setup {* add_rewrite_rule_back @{thm List.butlast_conv_take} *}
-setup {* add_rewrite_rule @{thm List.butlast_snoc} *}
+setup \<open>add_rewrite_arg_rule @{thm List.length_butlast}\<close>
+setup \<open>add_rewrite_rule @{thm List.nth_butlast}\<close>
+setup \<open>add_rewrite_rule_back @{thm List.butlast_conv_take}\<close>
+setup \<open>add_rewrite_rule @{thm List.butlast_snoc}\<close>
 lemma butlast_eval1 [rewrite]: "butlast [x] = []" by simp
 lemma butlast_eval2 [rewrite]: "butlast [x, y] = [x]" by simp
 lemma butlast_cons [rewrite]: "as \<noteq> [] \<Longrightarrow> butlast (a # as) = a # butlast as" by simp
 lemma butlast_append' [rewrite]: "bs \<noteq> [] \<Longrightarrow> butlast (as @ bs) = as @ butlast bs"
   by (simp add: butlast_append)
 
-setup {* add_rewrite_rule @{thm List.append_butlast_last_id} *}
+setup \<open>add_rewrite_rule @{thm List.append_butlast_last_id}\<close>
 lemma set_butlast_is_subset: "set (butlast xs) \<subseteq> set xs" by (simp add: in_set_butlastD subsetI)
-setup {* add_forward_arg1_prfstep @{thm set_butlast_is_subset} *}
+setup \<open>add_forward_arg1_prfstep @{thm set_butlast_is_subset}\<close>
 
 subsection \<open>List update\<close>
 
-setup {* register_wellform_data ("xs[i := x]", ["i < length xs"]) *}
-setup {* add_rewrite_arg_rule @{thm List.length_list_update} *}
-setup {* add_rewrite_rule @{thm List.nth_list_update_eq} *}
-setup {* add_rewrite_rule @{thm List.nth_list_update_neq} *}
-setup {* add_rewrite_rule @{thm List.nth_list_update} *}
+setup \<open>register_wellform_data ("xs[i := x]", ["i < length xs"])\<close>
+setup \<open>add_rewrite_arg_rule @{thm List.length_list_update}\<close>
+setup \<open>add_rewrite_rule @{thm List.nth_list_update_eq}\<close>
+setup \<open>add_rewrite_rule @{thm List.nth_list_update_neq}\<close>
+setup \<open>add_rewrite_rule @{thm List.nth_list_update}\<close>
 
 subsection \<open>take\<close>
 
-setup {* register_wellform_data ("take n xs", ["n \<le> length xs"]) *}
-setup {* add_prfstep_check_req ("take n xs", "n \<le> length xs") *}
+setup \<open>register_wellform_data ("take n xs", ["n \<le> length xs"])\<close>
+setup \<open>add_prfstep_check_req ("take n xs", "n \<le> length xs")\<close>
 
 lemma length_take [rewrite_arg]: "n \<le> length xs \<Longrightarrow> length (take n xs) = n" by simp
 lemma nth_take [rewrite]: "i < length (take n xs) \<Longrightarrow> take n xs ! i = xs ! i" by simp
 
-setup {* add_rewrite_rule @{thm List.take_0} *}
-setup {* add_rewrite_rule @{thm List.take_Suc_conv_app_nth} *}
+setup \<open>add_rewrite_rule @{thm List.take_0}\<close>
+setup \<open>add_rewrite_rule @{thm List.take_Suc_conv_app_nth}\<close>
 lemma take_length [rewrite]: "take (length xs) xs = xs" by simp
 
-setup {* add_forward_arg1_prfstep @{thm List.set_take_subset} *}
+setup \<open>add_forward_arg1_prfstep @{thm List.set_take_subset}\<close>
 
 lemma take_Suc [rewrite]: "Suc n \<le> length xs \<Longrightarrow> take (Suc n) xs = take n xs @ [nth xs n]"
   using Suc_le_lessD take_Suc_conv_app_nth by blast
 
-setup {* add_rewrite_rule @{thm List.take_update_cancel} *}
-setup {* add_rewrite_rule @{thm List.append_take_drop_id} *}
-setup {* add_rewrite_rule @{thm List.take_all} *}
+setup \<open>add_rewrite_rule @{thm List.take_update_cancel}\<close>
+setup \<open>add_rewrite_rule @{thm List.append_take_drop_id}\<close>
+setup \<open>add_rewrite_rule @{thm List.take_all}\<close>
 
 subsection \<open>drop\<close>
 
-setup {* add_rewrite_arg_rule @{thm List.length_drop} *}
+setup \<open>add_rewrite_arg_rule @{thm List.length_drop}\<close>
 lemma nth_drop [rewrite]:
   "i < length (drop n xs) \<Longrightarrow> drop n xs ! i = xs ! (n + i)" by simp
 
-setup {* add_rewrite_rule @{thm List.drop_0} *}
-setup {* add_rewrite_rule @{thm List.drop_all} *}
-setup {* add_rewrite_rule_back @{thm List.take_drop} *}
-setup {* add_rewrite_rule @{thm List.drop_drop} *}
+setup \<open>add_rewrite_rule @{thm List.drop_0}\<close>
+setup \<open>add_rewrite_rule @{thm List.drop_all}\<close>
+setup \<open>add_rewrite_rule_back @{thm List.take_drop}\<close>
+setup \<open>add_rewrite_rule @{thm List.drop_drop}\<close>
 
 subsection \<open>rev\<close>
 
-setup {* add_rewrite_arg_rule @{thm List.length_rev} *}
-setup {* fold add_rewrite_rule @{thms List.rev.simps} *}
-setup {* add_rewrite_rule @{thm List.rev_append} *}
-setup {* add_rewrite_rule @{thm List.rev_rev_ident} *}
+setup \<open>add_rewrite_arg_rule @{thm List.length_rev}\<close>
+setup \<open>fold add_rewrite_rule @{thms List.rev.simps}\<close>
+setup \<open>add_rewrite_rule @{thm List.rev_append}\<close>
+setup \<open>add_rewrite_rule @{thm List.rev_rev_ident}\<close>
 
 subsection \<open>filter\<close>
 
-setup {* fold add_rewrite_rule @{thms filter.simps} *}
-setup {* add_rewrite_rule @{thm filter_append} *}
-setup {* add_rewrite_rule_bidir @{thm rev_filter} *}
+setup \<open>fold add_rewrite_rule @{thms filter.simps}\<close>
+setup \<open>add_rewrite_rule @{thm filter_append}\<close>
+setup \<open>add_rewrite_rule_bidir @{thm rev_filter}\<close>
 
 subsection \<open>concat\<close>
 
-setup {* fold add_rewrite_rule @{thms concat.simps} *}
+setup \<open>fold add_rewrite_rule @{thms concat.simps}\<close>
 
 subsection \<open>mset\<close>
 
-setup {* add_rewrite_rule @{thm mset.simps(1)} *}
+setup \<open>add_rewrite_rule @{thm mset.simps(1)}\<close>
 lemma mset_simps_2 [rewrite]: "mset (a # x) = mset x + {#a#}" by simp
-setup {* add_rewrite_rule @{thm mset_append} *}
+setup \<open>add_rewrite_rule @{thm mset_append}\<close>
 
-setup {* add_rewrite_rule @{thm mset_eq_setD} *}
-setup {* add_rewrite_rule_cond @{thm in_multiset_in_set} [with_term "set ?xs"] *}
-setup {* add_rewrite_rule_back_cond @{thm in_multiset_in_set} [with_term "mset ?xs"] *}
-setup {* add_backward_prfstep @{thm Multiset.nth_mem_mset} *}
+setup \<open>add_rewrite_rule @{thm mset_eq_setD}\<close>
+setup \<open>add_rewrite_rule_cond @{thm in_multiset_in_set} [with_term "set ?xs"]\<close>
+setup \<open>add_rewrite_rule_back_cond @{thm in_multiset_in_set} [with_term "mset ?xs"]\<close>
+setup \<open>add_backward_prfstep @{thm Multiset.nth_mem_mset}\<close>
 
 lemma in_mset_conv_nth [resolve]: "x \<in># mset xs \<Longrightarrow> \<exists>i<length xs. x = xs ! i"
   by (metis in_multiset_in_set in_set_conv_nth)
 
 lemma hd_in_mset: "xs \<noteq> [] \<Longrightarrow> hd xs \<in># mset xs" by simp
-setup {* add_forward_prfstep_cond @{thm hd_in_mset} [with_term "hd ?xs", with_term "mset ?xs"] *}
+setup \<open>add_forward_prfstep_cond @{thm hd_in_mset} [with_term "hd ?xs", with_term "mset ?xs"]\<close>
 
 lemma last_in_mset: "xs \<noteq> [] \<Longrightarrow> last xs \<in># mset xs" by simp
-setup {* add_forward_prfstep_cond @{thm last_in_mset} [with_term "last ?xs", with_term "mset ?xs"] *}
+setup \<open>add_forward_prfstep_cond @{thm last_in_mset} [with_term "last ?xs", with_term "mset ?xs"]\<close>
 
 subsection \<open>Relationship between mset and set of lists\<close>
 
@@ -268,8 +268,8 @@ lemma mset_update' [rewrite]:
 
 subsection \<open>swap\<close>
 
-setup {* add_rewrite_rule @{thm mset_swap} *}
-setup {* add_rewrite_rule @{thm set_swap} *}
+setup \<open>add_rewrite_rule @{thm mset_swap}\<close>
+setup \<open>add_rewrite_rule @{thm set_swap}\<close>
 
 subsection \<open>upto lists\<close>
 
@@ -286,15 +286,15 @@ lemma list_nth [rewrite]: "i < length (list s n) \<Longrightarrow> (list s n) ! 
 
 subsection \<open>Splitting of lists\<close>
 
-setup {* add_resolve_prfstep @{thm split_list} *}
-setup {* add_backward_prfstep @{thm not_distinct_decomp} *}
+setup \<open>add_resolve_prfstep @{thm split_list}\<close>
+setup \<open>add_backward_prfstep @{thm not_distinct_decomp}\<close>
 
 subsection \<open>Finiteness\<close>
 
-setup {* add_resolve_prfstep @{thm finite_lists_length_le} *}
+setup \<open>add_resolve_prfstep @{thm finite_lists_length_le}\<close>
 
 subsection \<open>Cardinality\<close>
 
-setup {* add_rewrite_rule @{thm distinct_card} *}
+setup \<open>add_rewrite_rule @{thm distinct_card}\<close>
 
 end
