HOL/SepLogic/Union_Find_Impl.thy
@@ -116,6 +116,6 @@ lemma uf_union_rule [hoare_triple]:
    uf_union u i j
    <is_uf n (per_union R i j)>" by auto2
 
-setup {* del_prfstep_thm @{thm is_uf_def} *}
+setup \<open>del_prfstep_thm @{thm is_uf_def}\<close>
 
 end
